examples/ghc/theories/Axioms.v
@@ -1,0 +1,174 @@
+(* Disable notation conflict warnings *)
+Set Warnings "-notation-overridden".
+
+(* This file gathers and explains axioms about the GHC development. *)
+
+From mathcomp.ssreflect
+Require Import ssreflect ssrnat prime ssrbool.
+
+
+
+Require Import Coq.Lists.List.
+Import ListNotations.
+
+Require Import Coq.Classes.Morphisms. 
+
+Require Import GHC.Base.
+
+Require Import PrelNames.
+Require Import Id.
+Require Import Core.
+Require Import Unique.
+Require Import CoreFVs.
+
+Set Implicit Arguments.
+Unset Strict Implicit.
+Unset Printing Implicit Defensive.
+Set Bullet Behavior "Strict Subproofs".
+
+
+(**
+
+** Local uniques
+
+The Uniques in GHC are partitioned in classes, e.g. local variables have a different
+class than external names, which are different from data constructors and so on.
+
+The class is encoded in the upper 8 bits of the Unique. Our representation does not have 
+upper bits... and we hope we can make do with less details. For our proofs, it would suffice
+to axiomatize what we need:
+
+ * A predicate that distinguishes the uniques used for (module)-local variables, [isLocalUnique]
+ * An axiom stating that [uniqAway] always generates local uniques (see below).
+ * An axiom stating that some uniques are local: in particular, initExitJoinUnique.
+
+But in order to prove our invariants for concrete Core terms as dumped from GHC, we
+need the [isLocalUnique] function to compute. So hence it is a definition.
+
+*)
+
+
+(*
+
+From Unique.hs:
+
+Allocation of unique supply characters:
+        v,t,u : for renumbering value-, type- and usage- vars.
+        B:   builtin
+        C-E: pseudo uniques     (used in native-code generator)
+        X:   uniques derived by deriveUnique
+        _:   unifiable tyvars   (above)
+        0-9: prelude things below
+             (no numbers left any more..)
+        ::   (prelude) parallel array data constructors
+
+        other a-z: lower case chars for unique supplies.  Used so far:
+
+        d       desugarer
+        f       AbsC flattener
+        g       SimplStg
+        k       constraint tuple tycons
+        m       constraint tuple datacons
+        n       Native codegen
+        r       Hsc name cache
+        s       simplifier
+        z       anonymous sums
+*)
+
+Open Scope N_scope.
+Definition isLocalUnique  (u : Unique.Unique) : bool :=
+  (u == mkPreludeMiscIdUnique  0) (* The wild card key is local *)
+  || let '(c,i) := unpkUnique u in
+     negb (List.elem c &"B0123456789:kmnrz").
+
+
+(** [initExitJoinUnique] better be a local unique *)
+Axiom isLocalUnique_initExitJoinUnique:
+  isLocalUnique Unique.initExitJoinUnique = true.
+
+
+
+(** ** [uniqAway] axiomatization *)
+
+
+(* If uniqAway returns a variable with the same unique, 
+   it returns the same variable. *)      
+Axiom uniqAway_eq_same : forall v in_scope_set,
+    (uniqAway in_scope_set v == v) = true ->
+    (uniqAway in_scope_set v = v).
+
+(* The variable returned by uniqAway is fresh. *)
+Axiom uniqAway_lookupVarSet_fresh : forall v in_scope_set,
+    lookupVarSet (getInScopeVars in_scope_set) (uniqAway in_scope_set v) = None.
+
+
+(* Unique away preserves the classification of Vars. *)   
+Axiom isJoinId_maybe_uniqAway:
+  forall s v, 
+  isJoinId_maybe (uniqAway s v) = isJoinId_maybe v.
+
+(* See discussion of [isLocalUnique] above *)
+Axiom isLocalUnique_uniqAway:
+  forall iss v,
+  isLocalUnique (varUnique (uniqAway iss v)) = true.
+
+Axiom isLocalId_uniqAway:
+  forall iss v,
+  isLocalId (uniqAway iss v) = isLocalId v.
+
+Axiom isLocalVar_uniqAway:
+  forall iss v,
+  isLocalVar (uniqAway iss v) = isLocalVar v.
+
+Axiom isId_uniqAway:
+  forall iss v,
+    isId (uniqAway iss v) = isId v.
+
+Axiom isCoVar_uniqAway:
+  forall iss v,
+    isCoVar (uniqAway iss v) = isCoVar v.
+
+(* Variables have a unique cached inside.  This unique *should* be 
+   the same as the unique stored in the name of the variable. *)
+
+Axiom nameUnique_varName_uniqAway:
+  forall vss v,
+  Name.nameUnique (varName v) = varUnique v ->
+  Name.nameUnique (varName (uniqAway vss v)) = varUnique (uniqAway vss v).
+
+(**** *)
+
+(* NOTE: are these better as rewrites? Or as axioms? *)
+Axiom isJoinId_maybe_setIdOccInfo:
+  forall v occ_info, 
+  isJoinId_maybe (setIdOccInfo v occ_info) = isJoinId_maybe v.
+
+Axiom isJoinId_maybe_asJoinId:
+  forall v a,
+  isJoinId_maybe (asJoinId v a) = Some a.
+
+(** ** isLocalVar respects the GHC.Base.== equality for Vars  *)
+
+Definition RespectsVar (f :Var -> bool) :=
+    Proper ((fun x0 y : Var => x0 == y) ==> Logic.eq) f.
+
+Axiom RespectsVar_isLocalVar : RespectsVar isLocalVar.
+Hint Resolve RespectsVar_isLocalVar.
+
+(** ** Valid VarSets *)
+
+(* This property is an invariant of the VarSet/UniqFM type. We may want to either 
+   axiomatize it or add it to a sigma type in one of the definitions. *)
+
+Definition ValidVarSet (vs : VarSet) : Prop :=
+  forall v1 v2, lookupVarSet vs v1 = Some v2 -> (v1 == v2).
+
+Axiom ValidVarSet_Axiom : forall vs, ValidVarSet vs.
+
+
+(********************************* *)
+(* From: CoreFVs. Used in Exitify *)
+Axiom freeVarsOf_freeVars:
+  forall e,
+  dVarSetToVarSet (freeVarsOf (freeVars e)) = exprFreeVars e.
+
