examples/ghc/theories/FV.v
@@ -6,6 +6,7 @@ Require Import ssreflect ssrnat prime ssrbool eqtype.
 
 Require Import Core.
 Require Import FV.
+Require Import Proofs.Axioms.
 Require Import Proofs.ContainerAxioms.
 Require Import Proofs.VarSet.
 Require Import Proofs.VarSetFSet.
